src/lib/state/DY.Lib.State.Typed.fst
@@ -56,8 +56,8 @@ val typed_state_pred_label_pred_allow_inversion:
   Lemma
   (inversion (option a))
   [SMTPatOr [
-    [SMTPat (state_pred_label_can_flow p2 (tagged_state_pred_label_pred (typed_state_pred_label_pred p1)))];
-    [SMTPat (state_pred_label_can_flow (tagged_state_pred_label_pred (typed_state_pred_label_pred p1)) p2)];
+    [SMTPat (state_pred_label_pred_can_flow p2 (tagged_state_pred_label_pred (typed_state_pred_label_pred p1)))];
+    [SMTPat (state_pred_label_pred_can_flow (tagged_state_pred_label_pred (typed_state_pred_label_pred p1)) p2)];
   ]]
 let typed_state_pred_label_pred_allow_inversion #a #ps_a p1 p2 =
   allow_inversion (option a)
